% Part: first-order-logic 
% Chapter: axiomatic-deduction 
% Section: proving-things

\documentclass[../../include/open-logic-section]{subfiles}

\begin{document}

\olfileid{fol}{axd}{pro}

\olsection{Examples of \usetoken{P}{derivation}}

\begin{prop}
\ollabel{prop:easyproofs}
The following are !!{derivable}:
\begin{enumerate}
\item \ollabel{prop:easyproofs:trans}
\emph{Transitivity}: $\{!A \lif !B, !B \lif !C\} \Proves
  !A \lif !C$.
\item \ollabel{prop:easyproofs:refl}
  $\Proves !A \lif !A$. 
\end{enumerate}
\end{prop}

\begin{proof}
For part \olref{prop:easyproofs:trans}, the following instances
of \textbf{Ax1} and \textbf{Ax2} are needed:
\begin{align*}
  (!B \lif !C) & \lif (!A \lif (!B \lif !C)); \\
  (!A \lif (!B \lif !C)) & \lif ((!A \lif !B) \lif
    (!A \lif !C)).
\end{align*}
For part \olref{prop:easyproofs:refl}, consider the instance of
\textbf{Ax1}: $!A \lif ((!A \lif !A) \lif
!A)$ and distribute the outermost implication by \textbf{Ax2}.
\end{proof}

Let us show that $\lforall[x][!B] \Proves \lexists[x][!B]$
(where the !!{formula} on the right of the turnstile is just an
abbreviation for $\lnot \lforall[x][\lnot !B]$):

\begin{derivation}
 1. & $\lforall[x][\lnot !B] \lif \lnot \Subst{!B}{c}{x}$ &
 \textbf{Ax1}: $c$ !!{free for} $x$ in $\lnot !B$ \\
 2. &  $(\lforall[x][\lnot !B] \lif \lnot \Subst{!B}{c}{x}) \lif
 (\Subst{!B}{c}{x} \lif \lnot\lforall[x][\lnot !B]))$ & \textbf{Ax0}\\
 3. & $\Subst{!B}{c}{x} \lif \lnot\lforall[x][\lnot !B]$ & 1, 2, MP\\
 4. & $\lforall[x][!B] \lif \Subst{!B}{c}{x}$ & \textbf{Ax1}: $c$ free
 for $x$ in $!B$ \\
 5. & $\lforall[x][!B]$ & hyp. \\
 6. & $\Subst{!B}{c}{x}$ & 4, 5, MP \\
 7. & $\lnot \lforall[x][\lnot !B]$ & 3, 6, MP
\end{derivation}

\begin{prob} 
Show that the following hold by \emph{exhibiting}
!!{derivation}s from the axioms (i.e., without using meta-theoretic facts
such as Cut, Monotony, the Deduction Theorem, etc.): 
\begin{enumerate} 
\item $\{!A\lif !B, !B\lif !C\} \Proves !A\lif !C$;
\item $\Proves !A \lif !A$;
\item $\Proves \lnot !A \lif (!A \lif !B)$;
\item $\Proves !A \lif (\lnot !A \lif !B)$.
\end{enumerate} 
\end{prob}

\end{document}
