% part: intuitionistic-logic
% chapter: introduction
% section: bhk-interpretation

\documentclass[../../../include/open-logic-section]{subfiles}

\begin{document}

\olfileif{int}{int}{bhk}

\olsection{The Brouwer-Heyting-Kolmogorov Interpretation}

There is an informal constructive interpretation of the intuitionist
connectives, usually known as the Brouwer-Heyting-Kolmogorov
interpretation. Assuming our language ranges over natural numbers, it says:
\begin{enumerate}
\item We assume that we know what constitute a proof of an atomic
  statement.
\item A proof of $!A_1 \land !A_2$ is a pair $\tuple{M_1, M_2}$ where
  $M_1$ is a proof of~$!A_1$ and $M_2$ is a proof of $A_2$.
\item A proof of $!A_1 \lor !A_2$ is a pair $\tuple{s, M}$ where $s$
  is~$1$ and $M$ is a proof of~$!A_1$, or $s$ is~$2$ and $M$ is a
  proof of~$!A_2$.
\item A proof of $!A \lif !B$ is a function that converts a proof
  of~$!A$ into a proof of~$!B$.
\item There is no proof for~$\lfalse$ (absurdity).
\item $\lnot !A$ is defined as synonym for $!A \lif \lfalse$. That is,
  a proof of $\lnot !A$ is a function converting a proof of~$!A$ into
  a proof of~$\lfalse$.
\tagitem{FOL}{A proof of $\lforall[x][!A(x)]$ is a function that converts a
  natural number $n$ to a proof of~$!A(n)$.}{}
\tagitem{FOL}{A proof of $\lexists[x][!A(x)]$ is a pair $\tuple{n, M}$ where
  $n$ is a natural number, and $M$ is a proof of~$!A(n)$.}{}
\end{enumerate}

\begin{ex}
Take $\lnot 0=1$ for example. A proof of it is a function which, given
any proof of $0=1$ as input, provides a proof of~$\lfalse$ as
output. Of course, $\lfalse$ has no proof, which is not a problem as
no one can provide a proof of $0=1$ in the first place. Thus we may
use the identify function (or any other function) as the proof, and
our criteria for a function to be a proof (returning $\lfalse$ given a
proof of $0=1$) vacuously holds.
\end{ex}

General speaking, $\lnot !A$ means ``A proof of $!A$ is impossible''.

\begin{ex}
Let us prove $!A \lif \lnot \lnot !A$ for any proposition $!A$, which
is $!A \lif ((!A \lif \lfalse) \lif \lfalse)$. The proof should be a
function~$f$ that, given a proof~$M$ of $!A$, returns a proof~$f(M)$
of $(!A \lif \lfalse) \lif \lfalse$. Here is how~$f$ constructs the
proof of $(!A \lif \lfalse) \lif \lfalse$: What we need is a function
$g$ which, when given a proof~$h$ of $!A \lif \lfalse$ as input,
outputs a proof of~$\lfalse$. We can define $g$ as follows: apply the
input~$h$ to the proof~$M$ of $!A$ (that we received earlier). Since
the output of $h$ is a proof of $\lfalse$, $h(M)$ is a proof
of~$\lfalse$.
\end{ex}

Note in the above example we can't use the same trick we used when proving
$\lnot 0=1$, since it's possible that the skeptic of the proposition
indeed has the proof of $!A$ or $\lnot !A$. Is it possible that $!A$
and $\lnot !A$ are both provable? 

\begin{ex}
Let us prove $\lnot(!A \land \lnot !A)$, which is $(!A \land (!A \lif
\lfalse)) \lif \lfalse$. First we receive a proof of $!A \land (!A
\lif \lfalse)$ which should be a pair~$\tuple{M_1, M_2}$ whose first
element~$M_1$ is a proof of~$!A$ and the second is a proof~$M_2$ of
$!A \lif \lfalse$. Applying the second to the first, we get a proof
of~$\lfalse$ as required.
\end{ex}

\begin{ex}
Let us prove $((!A \land !B) \lif !C) \lif (!A \lif (!B \lif !C))$:
given $!A \land !B \lif !C$ we give $!A \lif !B \lif !C$, which we
construct as follows: given $!A$ we give $!B \lif !C$, which we
construct as follows: given $!B$ we give $!C$, which we construct as
follows: construct $!A \land !B$ from the given $!A$ and $!B$, pass it
to the given $!A \land !B \lif !C$ and we get $!C$ as required.
\end{ex}

Note how this is related to currying we introduced in lambda
calculus: if we consider the actual proof terms, we will find our
proof a function currying functions; the converse of the formula is also
provable (the proof is left to the reader) and corresponds to uncurrying.

The statement $!A \lor \lnot !A$ is called LEM (Law of Excluded
Middle). We can prove it for some specific $!A$(say,
$0=1$ or $0=0$), but not in general because the
intuitionistic disjunction requires a proof of either side, but there
are statements neither proved or refuted(say, Goldbach's conjecture as
of 2016). However, you can't refute LEM either: that is, $\lnot
\lnot (!A \lor \lnot !A)$.

\begin{ex}
Here is how we prove it: given $(!A \lor (!A \lif \lfalse))\lif
\lfalse$, we are expected to give $\lfalse$. We now try to construct
$!A \lor (!A \lif \lfalse)$ so we can apply the given function to get
$\lfalse$.

But wait, haven't we just established that $!A \lor (!A \lif \lfalse)$
is not provable in general? But note that we are in a position
different from the general case: now we have $(!A \lor (!A \lif
\lfalse))\lif \lfalse$ as premise, which is enough for us to derive
LEM: we will construct the right side of the disjunction, $!A \lif
\lfalse$: we are given $!A$ and expected to give $\lfalse$. Attention!
From $!A$ we can derive $!A \lor (!A \lif \lfalse)$; applying the
mentioned premise to it we get $\lfalse$, as required.
\end{ex}

This kind of proving soon gets too twisted to construct and understand;
we thus need a more formal language to construct such proofs.
\end{document}
