% Part: normal-modal-logic
% Chapter: syntax-and-semantics
% Section: substitution

\documentclass[../../../include/open-logic-section]{subfiles}

\begin{document}

\olfileid{mod}{syn}{sub}

\olsection{Simultaneous Substitution}

\begin{defn}\label{def:subst-inst}
  Where $!A$ is a modal !!{formula} all of whose !!{propositional
    variable}s are among $p_1$, \dots, $p_n$, and $!C_1$, \dots,
  $!C_n$ are also modal !!{formula}s, we define
  $\SSubst{!A}{\subst{!C_1}{p_1}, \dots, \subst{!C_n}{p_n}}$ as the
    result of simultaneously substituting each $!C_i$ for $p_i$ in
    $\!A$. Formally, this is a definition by induction on~$!A$:
  \begin{enumerate}
  \item If $!A$ is the !!{propositional variable}~$q$, then
    $\SSubst{!A}{\subst{!C_1}{p_1}, \dots, \subst{!C_n}{p_n}} = !C_i$
    if $Q$ is $p_i$ for some $i \le n$, and
    $\SSubst{!A}{\subst{!C_1}{p_1}, \dots, \subst{!C_n}{p_n}} = Q$
    otherwise.
  \item If $\!A = \lnot!B$, then $\SSubst{!A}{\subst{!C_1}{p_1},
    \dots, \subst{!C_n}{p_n}} = \lnot \SSubst{!B}{\subst{!C_1}{p_1},
    \dots, \subst{!C_n}{p_n}}$.
  \item If $!A = (!B \land !D)$, then
    \[\SSubst{!A}{\subst{!C_1}{p_1}, \dots, \subst{!C_n}{p_n}} =
    (\SSubst{!B}{\subst{!C_1}{p_1}, \dots, \subst{!C_n}{p_n}} \land
    \SSubst{!D}{\subst{!C_1}{p_1}, \dots, \subst{!C_n}{p_n}}).\]
  \item If $!A = (!B \lor !D)$, then
    \[\SSubst{!A}{\subst{!C_1}{p_1}, \dots, \subst{!C_n}{p_n}} =
    (\SSubst{!B}{\subst{!C_1}{p_1}, \dots, \subst{!C_n}{p_n}} \lor
    \SSubst{!D}{\subst{!C_1}{p_1}, \dots, \subst{!C_n}{p_n}}).\]
  \item If $!A = (!B \lif !D)$, then
    \[\SSubst{!A}{\subst{!C_1}{p_1}, \dots, \subst{!C_n}{p_n}} =
    (\SSubst{!B}{\subst{!C_1}{p_1}, \dots, \subst{!C_n}{p_n}} \lif
    \SSubst{!D}{\subst{!C_1}{p_1}, \dots, \subst{!C_n}{p_n}}).\]
  \item If $!A = (!B \liff !D)$, then
    \[\SSubst{!A}{\subst{!C_1}{p_1}, \dots, \subst{!C_n}{p_n}} =
    (\SSubst{!B}{\subst{!C_1}{p_1}, \dots, \subst{!C_n}{p_n}} \liff
    \SSubst{!D}{\subst{!C_1}{p_1}, \dots, \subst{!C_n}{p_n}}).\]
  \item If $!A = \Box !B$, then $\SSubst{!A}{\subst{!C_1}{p_1}, \dots,
    \subst{!C_n}{p_n}} = \Box \SSubst{!B}{\subst{!C_1}{p_1}, \dots,
    \subst{!C_n}{p_n}}$.
  \item If $!A = \Diamond !B$, then $\SSubst{!A}{\subst{!C_1}{p_1}, \dots,
    \subst{!C_n}{p_n}} = \Diamond \SSubst{!B}{\subst{!C_1}{p_1}, \dots,
    \subst{!C_n}{p_n}}$.
  \end{enumerate}
  The !!{formula} $\SSubst{!A}{\subst{!C_1}{p_1}, \dots,
    \subst{!C_n}{p_n}}$ is called a \emph{substitution instance}
  of~$!A$.
\end{defn}

\end{document}
